Work on formalizing Kozen's paper on SKAT
1. Defined flowcharts in Flowchart.thy (needs some polishing though)

1.1 Made flowcharts less polymorphic, athough they still need to be parameterised by an alphabet, which makes it hard to define certain things as types.

2. Defined a type for alphabets in Alphabet.thy

3. Defined traces build from atomic programs (aka atomic flowcharts) and have shown that they form a Quantale.

Carrier/Flowchart.thy
@@ -1,124 +1,79 @@
 theory Flowchart
-  imports Base
+  imports Alphabet
 begin
 
-record 'a alphabet =
-  symbols :: "'a set"
+datatype trm = var nat | app nat "trm list"
 
-locale alphabet = fixes \<Sigma> (structure)
-  assumes finite_symbols: "finite (symbols \<Sigma>)"
+datatype atomic_formula = app_rel nat "trm list"
 
-record 'a ranked_alphabet = "'a alphabet" +
-  arity :: "'a \<Rightarrow> nat"
-  funs :: "'a set"
-  rels :: "'a set"
-  outputs :: "nat set"
+fun wf_term :: "alphabet \<Rightarrow> trm \<Rightarrow> bool" where
+    "wf_term \<Sigma> (var _) = True"
+  | "wf_term \<Sigma> (app f xs) =
+       (length xs = arity \<Sigma> f \<and> f \<in> funs \<Sigma> \<and> (\<forall>x\<in>set xs. wf_term \<Sigma> x))"
 
-locale ranked_alphabet = alphabet +
-  assumes "funs \<Sigma> \<inter> rels \<Sigma> = {}"
-  and "funs \<Sigma> \<union> rels \<Sigma> = symbols \<Sigma>"
-  and "finite (outputs \<Sigma>)"
-  and "funs \<Sigma> \<noteq> {}"
-  and "rels \<Sigma> \<noteq> {}"
+fun wf_atomic_formula :: "alphabet \<Rightarrow> atomic_formula \<Rightarrow> bool" where
+    "wf_atomic_formula \<Sigma> (app_rel P xs) =
+       (length xs = arity \<Sigma> P \<and> P \<in> rels \<Sigma> \<and> (\<forall>x\<in>set xs. wf_term \<Sigma> x))"
 
-datatype 'a trm = var nat | app 'a "('a trm) list"
+datatype flowchart
+  = assignmenth nat trm
+  | assignment nat trm flowchart
+  | skiph
+  | skip flowchart
+  | undefh
+  | undef flowchart
+  | choicehh atomic_formula
+  | choicefh atomic_formula flowchart
+  | choicehf atomic_formula flowchart
+  | choiceff atomic_formula flowchart flowchart
 
-datatype 'a atomic_formula = app_rel 'a "('a trm) list"
+fun compose :: "flowchart \<Rightarrow> flowchart \<Rightarrow> flowchart" where
+    "compose (assignmenth x y) T = assignment x y T"
+  | "compose (assignment x y S) T = assignment x y (compose S T)"
+  | "compose skiph T = T"
+  | "compose (skip S) T = compose S T"
+  | "compose undefh T = undef T"
+  | "compose (undef S) T = undef (compose S T)"
+  | "compose (choicehh p) R = R"
+  | "compose (choicefh p S) R = choiceff p (compose S R) R"
+  | "compose (choicehf p T) R = choiceff p R (compose T R)"
+  | "compose (choiceff p S T) R = choiceff p (compose S R) (compose T R)"
 
-context ranked_alphabet
-begin
+lemma flowchart_assoc: "compose (compose S T) U = compose S (compose T U)" by (induct S, auto)
 
-  fun wf_term :: "'a trm \<Rightarrow> bool" where
-    "wf_term (var _) = True"
-  | "wf_term (app f xs) =
-      (length xs = arity \<Sigma> f \<and> f \<in> funs \<Sigma> \<and> (\<forall>x\<in>set xs. wf_term x))"
+lemma skiph_onel: "compose skiph T = T" by simp
 
-  definition wf_term_set :: "('a trm) set" where
-    "wf_term_set \<equiv> {x. wf_term x}"
+datatype expr
+  = e_assignment nat trm
+  | e_skip
+  | e_undef
+  | e_compose expr expr
+  | e_choicehh atomic_formula
+  | e_choicefh atomic_formula expr
+  | e_choicehf atomic_formula expr
+  | e_choiceff atomic_formula expr expr
 
-  lemma wf_var: "wf_term (var x)" by simp
+fun flowchart_to_expr :: "flowchart \<Rightarrow> expr" where
+    "flowchart_to_expr (assignmenth x y) = e_assignment x y"
+  | "flowchart_to_expr skiph = e_skip"
+  | "flowchart_to_expr undefh = e_undef"
+  | "flowchart_to_expr (assignment x y S ) = e_compose (e_assignment x y) (flowchart_to_expr S)"
+  | "flowchart_to_expr (skip S) = e_compose e_skip (flowchart_to_expr S)"
+  | "flowchart_to_expr (undef S) = e_compose e_undef (flowchart_to_expr S)"
+  | "flowchart_to_expr (choicehh p) = e_choicehh p"
+  | "flowchart_to_expr (choicefh p S) = e_choicefh p (flowchart_to_expr S)"
+  | "flowchart_to_expr (choicehf p T) = e_choicehf p (flowchart_to_expr T)"
+  | "flowchart_to_expr (choiceff p S T) = e_choiceff p (flowchart_to_expr S) (flowchart_to_expr T)"
 
-  fun wf_atomic_formula :: "'a atomic_formula \<Rightarrow> bool" where
-    "wf_atomic_formula (app_rel P xs) =
-      (length xs = arity \<Sigma> P \<and> P \<in> rels \<Sigma> \<and> (\<forall>x\<in>set xs. wf_term x))"
-
-end
-
-datatype 'a flowchart
-  = assignment nat "'a trm" "'a flowchart"
-  | skip "'a flowchart"
-  | halt
-  | undef "'a flowchart"
-  | choice "'a atomic_formula" "'a flowchart" "'a flowchart" ("IF _ THEN _ ELSE _")
-
-fun compose :: "'a flowchart \<Rightarrow> 'a flowchart \<Rightarrow> 'a flowchart" (infixl ";" 55) where
-    "compose (assignment x y S) T = assignment x y (S ; T)"
-  | "compose (skip S) T = (S ; T)"
-  | "compose halt T = T"
-  | "compose (undef S) T = undef (S ; T)"
-  | "compose (IF p THEN S ELSE T) R = IF p THEN (S ; R) ELSE (T ; R)"
-
-lemma compose_assoc: "(S ; T) ; U = S ; (T ; U)"
-  by (induct S, auto)
-
-definition ASSIGN :: "nat \<Rightarrow> 'a trm \<Rightarrow> 'a flowchart" (infix ":=" 80) where
-  "ASSIGN x y = assignment x y halt"
-
-definition SKIP :: "'a flowchart" where
-  "SKIP = skip halt"
-
-definition UNDEFINED :: "'a flowchart" where
-  "UNDEFINED = undef halt"
-
-definition atomic_programs :: "'a flowchart set" where
-  "atomic_programs \<equiv> {SKIP, UNDEFINED} \<union> {a. \<exists>x y. a = x := y}"
-
-lemma assign_compose: "x := y ; S = assignment x y S"
-  by (auto simp add: ASSIGN_def)
-
-inductive_set programs :: "'a flowchart set" where
-  atomic [intro]: "S \<in> atomic_programs \<Longrightarrow> S \<in> programs"
-| composition [intro]: "\<lbrakk>S \<in> programs; T \<in> programs\<rbrakk> \<Longrightarrow> S ; T \<in> programs"
-| choice [intro]: "\<lbrakk>S \<in> programs; T \<in> programs\<rbrakk> \<Longrightarrow> IF P THEN S ELSE T \<in> programs"
-
-lemma "SKIP ; T = T"
-  by (metis SKIP_def compose.simps(2) compose.simps(3))
-
-lemma halt_not_atomic: "halt \<notin> atomic_programs"
-  by (auto simp add: atomic_programs_def SKIP_def UNDEFINED_def ASSIGN_def)
-
-lemma any_undef_not_atomic: "S \<noteq> halt \<Longrightarrow> undef S \<notin> atomic_programs"
-  by (auto simp add: atomic_programs_def SKIP_def UNDEFINED_def ASSIGN_def)
-
-lemma any_skip_not_atomic: "S \<noteq> halt \<Longrightarrow> skip S \<notin> atomic_programs"
-  by (auto simp add: atomic_programs_def SKIP_def UNDEFINED_def ASSIGN_def)
-
-lemma halt_not_program: "halt \<notin> programs" sorry
-
-lemma "T \<in> programs \<Longrightarrow> T ; SKIP = T"
-  apply (induct T rule: programs.induct)
-  
-  apply auto
-  
-  
-  
-  
-
-context ranked_alphabet
-begin
-
-  fun wf_flowchart :: "'a flowchart \<Rightarrow> bool" where
-    "wf_flowchart (assignment x y S) = (wf_term y \<and> wf_flowchart S)"
-  | "wf_flowchart (skip S) = wf_flowchart S"
-  | "wf_flowchart halt = True"
-  | "wf_flowchart connection = True"
-  | "wf_flowchart (undef S) = wf_flowchart S"
-  | "wf_flowchart (IF p THEN S ELSE T) = (wf_flowchart S \<and> wf_flowchart T)"
-
-  lemma compose_wf: "\<lbrakk>wf_flowchart S; wf_flowchart T\<rbrakk> \<Longrightarrow> wf_flowchart (S ; T)"
-    by (induct S, simp_all)
-
-end
+fun expr_to_flowchart :: "expr \<Rightarrow> flowchart" where
+    "expr_to_flowchart (e_assignment x y) = assignmenth x y"
+  | "expr_to_flowchart e_skip = skiph"
+  | "expr_to_flowchart e_undef = undefh"
+  | "expr_to_flowchart (e_compose S T) = compose (expr_to_flowchart S) (expr_to_flowchart T)"
+  | "expr_to_flowchart (e_choicehh p) = choicehh p"
+  | "expr_to_flowchart (e_choicefh p S) = choicefh p (expr_to_flowchart S)"
+  | "expr_to_flowchart (e_choicehf p T) = choicehf p (expr_to_flowchart T)"
+  | "expr_to_flowchart (e_choiceff p S T) = choiceff p (expr_to_flowchart S) (expr_to_flowchart T)"
 
 fun ntuples :: "'a set \<Rightarrow> nat \<Rightarrow> ('a list) set" ("_\<^bsup>_\<^esup>") where
   "X\<^bsup>0\<^esup> = {[]}"
@@ -164,154 +119,264 @@ proof (auto simp add: ftype_def)
     by (induct xs, simp_all add: fplus_def)
 qed
 
-record 'a interp = "'a partial_object" +
-  fun_map :: "'a \<Rightarrow> 'a list \<Rightarrow> 'a"
-  rel_map :: "'a \<Rightarrow> 'a relation"
-  null :: "'a"
+record interp =
+  fun_map :: "nat \<Rightarrow> nat list \<Rightarrow> nat"
+  rel_map :: "nat \<Rightarrow> nat relation"
+  null :: "nat"
 
-record 'a frame =
-  alph :: "'a ranked_alphabet" ("\<Sigma>1\<index>")
-  ip :: "'a interp" ("D1\<index>")
+locale frame =
+  fixes \<Sigma>l :: "alphabet"
+  and Dl :: "interp"
+  assumes fun_meaning: "f \<in> funs \<Sigma>l \<Longrightarrow> fun_map Dl f : \<nat>\<^bsup>arity \<Sigma>l f\<^esup> \<rightarrow> \<nat>"
+  and rel_meaning: "P \<in> rels \<Sigma>l \<Longrightarrow> rel_map Dl P \<subseteq> \<nat>\<^bsup>arity \<Sigma>l f\<^esup>"
 
-locale frame = fixes \<Theta> (structure)
-  assumes is_ranked_alphabet: "ranked_alphabet \<Sigma>1"
-  and null_closed: "null D1 \<in> carrier D1"
-  and fun_meaning: "f \<in> funs \<Sigma>1 \<Longrightarrow> fun_map D1 f : (carrier D1)\<^bsup>arity \<Sigma>1 f\<^esup> \<rightarrow> carrier D1"
-  and rel_meaning: "P \<in> rels \<Sigma>1 \<Longrightarrow> rel_map D1 P \<subseteq> (carrier D1)\<^bsup>arity \<Sigma>1 f\<^esup>"
+datatype mem = mem "nat \<Rightarrow> nat"
+             | undefined_mem
 
-sublocale frame \<subseteq> ranked_alphabet where \<Sigma> = \<Sigma>1 by (rule is_ranked_alphabet)
+datatype ('a, 'b) either = Left 'a | Right 'b
+
+definition emp :: "interp \<Rightarrow>  mem" where
+  "emp D = mem (\<lambda>n. null D)"
 
 context frame
 begin
 
-  fun eval_term :: "(nat \<Rightarrow> 'a) \<Rightarrow> 'a trm \<Rightarrow> 'a" where
+  fun eval_term :: "(nat \<Rightarrow> nat) \<Rightarrow> trm \<Rightarrow> nat" where
     "eval_term var_map (var x) = var_map x"
-  | "eval_term var_map (app f xs) = fun_map D1 f (map (eval_term var_map) xs)"
+  | "eval_term var_map (app f xs) = fun_map Dl f (map (eval_term var_map) xs)"
 
   lemma wf_term_induction:
-    "\<lbrakk>wf_term t; \<And>n. P (var n); \<And>f xs. \<lbrakk>f \<in> funs \<Sigma>1; length xs = arity \<Sigma>1 f; \<And>x. x \<in> set xs \<Longrightarrow> P x\<rbrakk> \<Longrightarrow> P (app f xs)\<rbrakk> \<Longrightarrow> P t"
+    "\<lbrakk>wf_term \<Sigma>l t; \<And>n. P (var n); \<And>f xs. \<lbrakk>f \<in> funs \<Sigma>l; length xs = arity \<Sigma>l f; \<And>x. x \<in> set xs \<Longrightarrow> P x\<rbrakk> \<Longrightarrow> P (app f xs)\<rbrakk> \<Longrightarrow> P t"
     by (induct t rule: wf_term.induct, auto)
 
   lemma eval_term_closed:
-    assumes var_map_type: "var_map : \<nat> \<rightarrow> carrier D1"
-    and wft: "wf_term t"
-    shows "eval_term var_map t : carrier D1"
+    assumes var_map_type: "var_map : \<nat> \<rightarrow> \<nat>"
+    and wft: "wf_term \<Sigma>l t"
+    shows "eval_term var_map t : \<nat>"
     apply (induct t rule: wf_term_induction)
     apply (metis wft)
     apply (simp_all)
     apply (insert var_map_type, simp add: Nats_def)
-    apply (metis UNIV_I ftype_pred)
-    apply (subgoal_tac "map (eval_term var_map) xs \<in> (carrier D1)\<^bsup>length xs\<^esup>")
+    apply (subgoal_tac "map (eval_term var_map) xs \<in> \<nat>\<^bsup>length xs\<^esup>")
     apply (metis ftype_pred fun_meaning)
     apply (simp add: ntp1[symmetric])
     by auto
 
-  fun eval_pred :: "(nat \<Rightarrow> 'a) \<Rightarrow> 'a atomic_formula \<Rightarrow> bool" where
-    "eval_pred var_map (app_rel P xs) \<longleftrightarrow> map (eval_term var_map) xs \<in> rel_map D1 P"
+  fun eval_pred :: "(nat \<Rightarrow> nat) \<Rightarrow> atomic_formula \<Rightarrow> bool" where
+    "eval_pred var_map (app_rel P xs) \<longleftrightarrow> map (eval_term var_map) xs \<in> rel_map Dl P"
 
-  definition emp :: "nat \<Rightarrow> 'a" where
-    "emp n = null D1"
+  fun step_flowchart :: "(mem \<times> flowchart) \<Rightarrow> (mem, (mem \<times> flowchart)) either" where
+      "step_flowchart (mem vm, (assignmenth x y)) = Left (mem (\<lambda>z. if z=x then eval_term vm y else vm z))"
+    | "step_flowchart (mem vm, (assignment x y S)) = Right (mem (\<lambda>z. if z=x then eval_term vm y else vm z), S)"
+    | "step_flowchart (m, skiph) = Left m"
+    | "step_flowchart (m, skip S) = Right (m, S)"
+    | "step_flowchart (_, undefh) = Left undefined_mem"
+    | "step_flowchart (_, undef S) = Left undefined_mem"
+    | "step_flowchart (m, choicehh _) = Left m"
+    | "step_flowchart (mem vm, choicefh p S) = Right (mem vm, if eval_pred vm p then S else skiph)"
+    | "step_flowchart (mem vm, choicehf p T) = Right (mem vm, if eval_pred vm p then skiph else T)"
+    | "step_flowchart (mem vm, choiceff p S T) = Right (mem vm, if eval_pred vm p then S else T)"
+    | "step_flowchart (undefined_mem, _) = Left undefined_mem"
 
-  fun eval_flowchart :: "((nat \<Rightarrow> 'a) \<times> 'a flowchart) \<Rightarrow> ((nat \<Rightarrow> 'a) \<times> 'a flowchart)" where
-    "eval_flowchart (vm, (assignment x y S)) = eval_flowchart ((\<lambda>z. if z=x then eval_term vm y else vm z), S)"
-  | "eval_flowchart (vm, (skip S)) = eval_flowchart (vm, S)"
-  | "eval_flowchart (vm, halt) = (vm, halt)"
-  | "eval_flowchart (vm, connection) = (vm, connection)"
-  | "eval_flowchart (vm, undef S) = (emp, undef S)"
-  | "eval_flowchart (vm, IF P THEN S ELSE T) = eval_flowchart (vm, if eval_pred vm P then S else T)"
+  fun eval_flowchart :: "(mem \<times> flowchart) \<Rightarrow> mem" where
+      "eval_flowchart (mem vm, (assignmenth x y)) = mem (\<lambda>z. if z=x then eval_term vm y else vm z)"
+    | "eval_flowchart (mem vm, (assignment x y S)) = eval_flowchart (mem (\<lambda>z. if z=x then eval_term vm y else vm z), S)"
+    | "eval_flowchart (m, skiph) = m"
+    | "eval_flowchart (m, skip S) = eval_flowchart (m, S)"
+    | "eval_flowchart (_, undefh) = undefined_mem"
+    | "eval_flowchart (_, undef S) = undefined_mem"
+    | "eval_flowchart (m, choicehh _) = m"
+    | "eval_flowchart (mem vm, choicefh p S) = eval_flowchart (mem vm, if eval_pred vm p then S else skiph)"
+    | "eval_flowchart (mem vm, choicehf p T) = eval_flowchart (mem vm, if eval_pred vm p then skiph else T)"
+    | "eval_flowchart (mem vm, choiceff p S T) = eval_flowchart (mem vm, if eval_pred vm p then S else T)"
+    | "eval_flowchart (undefined_mem, _) = undefined_mem"
 
-  lemma "eval_flowchart (z, SKIP ; S) = eval_flowchart (z, S)"
-    by (simp add: SKIP_def)
+  function eval_flowchart_var :: "(mem \<times> flowchart) \<Rightarrow> mem" where
+      "eval_flowchart_var (m, S) = (case step_flowchart (m, S) of
+                                      (Left m) \<Rightarrow> m
+                                    | (Right (m, S')) \<Rightarrow> eval_flowchart_var (m, S'))"
+    by (pat_completeness, auto)
+    termination sorry (* TODO: Prove termination *)
 
-  lemma "fst (eval_flowchart (z, S ; SKIP)) = fst (eval_flowchart (z, S))"
-    by (induct S arbitrary: z, auto simp add: SKIP_def)
+  lemma "eval_flowchart (m, S) = eval_flowchart_var (m, S)"
+  proof -
+    have"\<And>vm. eval_flowchart (mem vm, S) = eval_flowchart_var (mem vm, S)"
+      by (induct S arbitrary: vm, auto)
+    moreover have "eval_flowchart (undefined_mem, S) = eval_flowchart_var (undefined_mem, S)"
+      by (induct S, auto)
+    ultimately show ?thesis
+      by (metis mem.exhaust)
+  qed
 
-  lemma "fst (eval_flowchart (z, UNDEFINED ; S)) = fst (eval_flowchart (z, UNDEFINED))"
-    by (induct S arbitrary: z, auto simp add: UNDEFINED_def)
+  lemma eval_skiph_onel: "eval_flowchart (m, compose skiph S) = eval_flowchart (m, S)" by auto
 
-  lemma "S \<in> programs \<Longrightarrow> fst (eval_flowchart (z, S ; UNDEFINED)) = emp"
-    apply (induct S arbitrary: z)
-    apply (auto simp add: UNDEFINED_def)
-    apply (subgoal_tac "S \<in> programs")
-    apply auto
-    apply (subgoal_tac "nat := trm ; S \<in> programs")
-    apply (simp add: compose_def)
-    
-    
-    try
-    
-    nitpick
-    
+  lemma eval_skiph_oner: "eval_flowchart (m, compose S skiph) = eval_flowchart (m, S)"
+  proof -
+    have "\<And>vm. eval_flowchart (mem vm, compose S skiph) = eval_flowchart (mem vm, S)"
+      by (induct S arbitrary: z, auto)
+    moreover have "eval_flowchart (undefined_mem, compose S skiph) = eval_flowchart (undefined_mem, S)"
+      by (induct S, auto)
+    ultimately show ?thesis
+      by (metis mem.exhaust)
+  qed
 
-  lemma "fst (eval_flowchart (emp, T)) = fst (eval_flowchart (emp, U)) \<Longrightarrow> fst (eval_flowchart (emp, S ; T)) = fst (eval_flowchart (emp, S ; U))"
-    apply (induct S)
-    apply auto
-    apply blast
-    
-    
-    defer
-    nitpick
-nitpick [non_std, show_all]
-    
-    apply (cases "z = nat")
-    sledgehammer
-    apply (simp add: 
+  lemma eval_undefh_zerol: "eval_flowchart (m, compose undefh S) = eval_flowchart (m, undefh)" by auto
+
+  lemma eval_undefh_zeror: "eval_flowchart (m, compose S undefh) = eval_flowchart (m, undefh)"
+  proof -
+    have "\<And>vm. eval_flowchart (mem vm, compose S undefh) = eval_flowchart (mem vm, undefh)"
+      by (induct S arbitrary: z, auto)
+    moreover have "eval_flowchart (undefined_mem, compose S undefh) = eval_flowchart (undefined_mem, undefh)"
+      by (induct S, auto)
+    ultimately show ?thesis
+      by (metis mem.exhaust)
+  qed
+
+  lemma eval_undefined_mem: "eval_flowchart (undefined_mem, T) = undefined_mem" by (induct T, auto)
+
+  lemma eval_compose: "eval_flowchart (m, compose S T) = eval_flowchart (eval_flowchart (m, S), T)"
+  proof -
+    have "\<And>vm. eval_flowchart (mem vm, compose S T) = eval_flowchart (eval_flowchart (mem vm, S), T)"
+      apply (induct S, auto, induct T, auto, induct T, auto)
+      by (metis skiph_onel eval_flowchart.simps(3))
+    moreover have "eval_flowchart (undefined_mem, compose S T) = eval_flowchart (eval_flowchart (undefined_mem, S), T)"
+      by (simp add: eval_undefined_mem)
+    ultimately show ?thesis
+      by (metis mem.exhaust)
+  qed
 
 end
 
-definition empty :: "'a interp \<Rightarrow> nat \<Rightarrow> 'a" where
-  "empty D n = null D"
+typedef 'a nset = "{X::'a set. X \<noteq> {}}"
+  by (metis (lifting, full_types) Collect_empty_eq ex_in_conv)
 
-definition equivalent_scheme :: "'a ranked_alphabet \<Rightarrow> 'a flowchart \<Rightarrow> 'a flowchart \<Rightarrow> bool" where
-  "equivalent_scheme \<Sigma> S T \<equiv> (\<forall>D::'a interp. frame \<lparr>alph = \<Sigma>, ip = D\<rparr> \<longrightarrow> frame.eval_flowchart \<lparr>alph = \<Sigma>, ip = D\<rparr> (empty D, S) = frame.eval_flowchart \<lparr>alph = \<Sigma>, ip = D\<rparr> (empty D, T))"
-
-lemma assumes eq_ST: "equivalent_scheme \<Sigma> S T" shows "equivalent_scheme \<Sigma> (S 
-; U) (T; U)"
-  apply (auto simp add: equivalent_scheme_def)
-  apply (induct U)
-  
-
-  apply (insert frame.wf_term_induction[of "\<lparr>alph = \<Sigma>, ip = D\<rparr>"])
-  apply (auto simp add: equivalent_scheme_def)
-
-
-lemma
-  assumes eq_UV: "equivalent_scheme \<Sigma> U V"
-  shows "equivalent_scheme \<Sigma> (S ; U) (S ; V)"
-  apply (induct S, simp_all add: equivalent_scheme_def, auto)
-  apply (auto simp add: equivalent_scheme_def)
-  
-  
-
-record 'a equivalence_relation = "'a partial_object" +
-  eq :: "'a \<Rightarrow> 'a \<Rightarrow> bool" (infix "~\<index>" 50)
-
-locale equivalence_relation = fixes A (structure)
-  assumes refl: "x \<in> carrier A \<Longrightarrow> x ~ x"
-  and sym: "\<lbrakk>x \<in> carrier A; y \<in> carrier A; x ~ y\<rbrakk> \<Longrightarrow> y ~ x"
-  and trans: "\<lbrakk>x \<in> carrier A; y \<in> carrier A; z \<in> carrier A; x ~ y; y ~ z\<rbrakk> \<Longrightarrow> x ~ z"
+locale alph =
+  fixes \<Sigma>l :: alphabet
+  and outputs :: "nat set"
 
 begin
 
-  definition canonical_projection_map :: "'a \<Rightarrow> 'a set" ("\<pi>") where
-    "\<pi> x \<equiv> {y. y \<in> carrier A \<and> x ~ y}"
-
-  lemma cpm_closed: "x \<in> carrier A \<Longrightarrow> \<pi> x \<subseteq> carrier A"
-    by (auto simp add: canonical_projection_map_def)
-
-  definition quotient :: "'a set set" where
-    "quotient \<equiv> {\<pi> x|x. x \<in> carrier A}"
+  definition equivalent_scheme :: "flowchart \<Rightarrow> flowchart \<Rightarrow> bool" where
+    "equivalent_scheme S T \<equiv> (\<forall>D m. frame \<Sigma>l D \<longrightarrow>
+      frame.eval_flowchart D (m, S) = frame.eval_flowchart D (m, T))"
 
 end
 
-definition frel :: "'a ranked_alphabet \<Rightarrow> ('a flowchart) equivalence_relation" where
-  "frel \<Sigma> \<equiv> \<lparr>carrier = UNIV, eq = equivalent_scheme \<Sigma>\<rparr>"
+type_synonym flow = "flowchart set"
 
-lemma frel_eq: "equivalence_relation (frel \<Sigma>)"
-  by (default, simp_all add: equivalent_scheme_def frel_def)
+context alph begin
 
-definition fquotient :: "'a ranked_alphabet \<Rightarrow> 'a flowchart set set" where
-  "fquotient \<Sigma> = equivalence_relation.quotient (frel \<Sigma>)"
+  definition cpm :: "flowchart \<Rightarrow> flow" ("\<pi>") where
+    "\<pi> s = {t. equivalent_scheme s t}"
 
-lemma "\<lbrakk>equivalence_relation \<lparr>carrier = X, eq = eq1\<rparr>; Y \<subseteq> X\<rbrakk> \<Longrightarrow> equivalence_relation \<lparr>carrier = Y, eq = eq1\<rparr>"
-  by (simp add: equivalence_relation_def, safe, fast+)
+  lemma scheme_refl [intro]: "equivalent_scheme s s"
+    by (simp add: equivalent_scheme_def)
+
+  lemma scheme_sym [sym]: "equivalent_scheme s t \<Longrightarrow> equivalent_scheme t s"
+    by (simp add: equivalent_scheme_def)
+
+  lemma scheme_trans [trans]: "\<lbrakk>equivalent_scheme s t; equivalent_scheme t u\<rbrakk> \<Longrightarrow> equivalent_scheme s u"
+    by (simp add: equivalent_scheme_def)
+
+  lemma cpm_equiv [simp]: "\<pi> s = \<pi> t \<longleftrightarrow> equivalent_scheme s t"
+    by (smt Collect_cong scheme_refl scheme_sym scheme_trans cpm_def mem_Collect_eq)
+
+  lemma in_cpm: "s \<in> \<pi> s"
+    by (auto simp add: cpm_def)
+
+  lemma cpm_not_empty: "\<pi> s \<noteq> {}"
+    by (metis empty_iff in_cpm)
+
+  lemma cpm1: "\<not> equivalent_scheme s t \<Longrightarrow> s \<notin> \<pi> t"
+    by (auto simp add: cpm_def, metis scheme_sym)
+
+  lemma cpm2: "\<not> equivalent_scheme s t \<Longrightarrow> t \<notin> \<pi> s"
+    by (metis scheme_sym cpm1)
+
+  definition scheme_compose :: "flow \<Rightarrow> flow \<Rightarrow> flow" (infixr ";" 80) where
+    "S ; T \<equiv> {U. \<exists>s\<in>S. \<exists>t\<in>T. equivalent_scheme U (compose s t)}"
+
+  definition flows :: "flow set" where
+    "flows \<equiv> {S. \<exists>s. S = \<pi> s}"
+
+  lemma compose_eq1: "equivalent_scheme s t \<Longrightarrow> equivalent_scheme (compose s u) (compose t u)"
+    by (simp add: equivalent_scheme_def frame.eval_compose)
+
+  lemma compose_eq2: "equivalent_scheme t u \<Longrightarrow> equivalent_scheme (compose s t) (compose s u)"
+    by (simp add: equivalent_scheme_def frame.eval_compose)
+
+  lemma compose_prop: "\<pi> s ; \<pi> t = \<pi> (compose s t)"
+    apply (auto simp add: cpm_def scheme_compose_def)
+    apply (smt compose_eq1 compose_eq2 scheme_sym scheme_trans)
+    by (metis scheme_refl scheme_sym)
+
+  lemma compose_flows: "\<lbrakk>S \<in> flows; T \<in> flows\<rbrakk> \<Longrightarrow> S ; T \<in> flows"
+    apply (auto simp add: flows_def)
+    apply (rule_tac x = "compose s sa" in exI)
+    by (simp add: compose_prop)
+
+  lemma compose_assoc:
+    assumes Sf: "S \<in> flows" and Tf: "T \<in> flows" and Uf: "U \<in> flows"
+    shows "(S ; T) ; U = S ; (T ; U)"
+  proof -
+    obtain s t u where Ss: "S = \<pi> s" and Tt: "T = \<pi> t" and Uu: "U = \<pi> u"
+      by (insert Sf Tf Uf, auto simp add: flows_def)
+    have "(S ; T) ; U = (\<pi> s; \<pi> t) ; \<pi> u"
+      by (simp add: Ss Tt Uu)
+    also have "... = \<pi> (compose (compose s t) u)"
+      by (simp add: compose_prop)
+    also have "... = \<pi> (compose s (compose t u))"
+      by (simp add: flowchart_assoc)
+    also have "... = \<pi> s ; (\<pi> t ; \<pi> u)"
+      by (simp add: compose_prop[symmetric])
+    also have "... = S ; (T ; U)"
+      by (metis Ss Tt Uu)
+    finally show ?thesis .
+  qed
+
+  definition SKIP :: flow where
+    "SKIP \<equiv> \<pi> skiph"
+
+  lemma SKIP_flows: "SKIP \<in> flows"
+    by (auto simp add: flows_def SKIP_def)
+
+  lemma SKIP_onel: assumes Sf: "S \<in> flows" shows "SKIP ; S = S"
+  proof -
+    obtain s where Ss: "S = \<pi> s" by (insert Sf, auto simp add: flows_def)
+    thus ?thesis
+      by (simp add: SKIP_def compose_prop)
+  qed
+
+  lemma SKIP_oner: assumes Sf: "S \<in> flows" shows "S ; SKIP = S"
+  proof -
+    obtain s where Ss: "S = \<pi> s" by (insert Sf, auto simp add: flows_def)
+    thus ?thesis
+      apply (auto simp add: SKIP_def compose_prop equivalent_scheme_def)
+      by (metis frame.eval_skiph_oner)
+  qed
+
+  definition UNDEFINED :: flow where
+    "UNDEFINED \<equiv> \<pi> undefh"
+
+  lemma UNDEFINED_flows: "UNDEFINED \<in> flows"
+    by (auto simp add: flows_def UNDEFINED_def)
+
+  lemma UNDEFINED_zerol: assumes Sf: "S \<in> flows" shows "UNDEFINED ; S = UNDEFINED"
+  proof -
+    obtain s where Ss: "S = \<pi> s" by (insert Sf, auto simp add: flows_def)
+    thus ?thesis
+      apply (auto simp add: UNDEFINED_def compose_prop equivalent_scheme_def)
+      by (metis compose.simps(5) frame.eval_undefh_zerol)
+  qed
+
+  lemma UNDEFINED_zeror: assumes Sf: "S \<in> flows" shows "S ; UNDEFINED = UNDEFINED"
+  proof -
+    obtain s where Ss: "S = \<pi> s" by (insert Sf, auto simp add: flows_def)
+    thus ?thesis
+      apply (auto simp add: UNDEFINED_def compose_prop equivalent_scheme_def)
+      by (metis frame.eval_undefh_zeror)
+  qed
+
+end
+
+end
