Carrier/Alphabet.thy
@@ -1,0 +1,72 @@
+theory Alphabet
+  imports Base
+begin
+
+record alphabet_tuple =
+  alphabet_symbols :: "nat set"
+  alphabet_arity :: "nat \<Rightarrow> nat"
+  alphabet_funs :: "nat set"
+  alphabet_rels :: "nat set"
+
+definition binary_alphabet_tuple :: "alphabet_tuple" where
+  "binary_alphabet_tuple = \<lparr> alphabet_symbols = {0, 1}
+                           , alphabet_arity = (\<lambda>x. 0)
+                           , alphabet_funs = {0}
+                           , alphabet_rels = {1}
+                           \<rparr>"
+
+typedef alphabet = "{\<Sigma>::alphabet_tuple. finite (alphabet_symbols \<Sigma>)
+                                      \<and> alphabet_funs \<Sigma> \<inter> alphabet_rels \<Sigma> = {}
+                                      \<and> alphabet_funs \<Sigma> \<union> alphabet_rels \<Sigma> = alphabet_symbols \<Sigma>
+                                      \<and> alphabet_funs \<Sigma> \<noteq> {} \<and> alphabet_rels \<Sigma> \<noteq> {}}"
+  by (rule_tac x = "binary_alphabet_tuple" in exI, auto simp add: binary_alphabet_tuple_def)
+
+definition symbols :: "alphabet \<Rightarrow> nat set" where
+  "symbols = alphabet_symbols \<circ> Rep_alphabet"
+
+definition arity :: "alphabet \<Rightarrow> nat \<Rightarrow> nat" where
+  "arity = alphabet_arity \<circ> Rep_alphabet"
+
+definition funs :: "alphabet \<Rightarrow> nat set" where
+  "funs = alphabet_funs \<circ> Rep_alphabet"
+
+definition rels :: "alphabet \<Rightarrow> nat set" where
+  "rels = alphabet_rels \<circ> Rep_alphabet"
+
+declare Rep_alphabet_inverse [simp]
+
+(* TODO: These should hardly require sledgehammer to solve... *)
+
+lemma symbols_finite: "finite (symbols \<Sigma>)"
+  apply (simp add: symbols_def)
+  apply (rule Abs_alphabet_induct)
+  apply (auto simp add: alphabet_def)
+  by (smt CollectE Rep_alphabet alphabet_def)
+
+lemma funs_rels_disjoint: "funs \<Sigma> \<inter> rels \<Sigma> = {}"
+  apply (simp add: funs_def rels_def)
+  apply (rule Abs_alphabet_induct)
+  apply (auto simp add: alphabet_def)
+  by (smt Abs_alphabet_cases Abs_alphabet_inverse CollectI Collect_empty_eq Collect_mem_eq alphabet_def disjoint_iff_not_equal)
+
+lemma symbol_fun_or_rel: "funs \<Sigma> \<union> rels \<Sigma> = symbols \<Sigma>"
+  apply (simp add: funs_def rels_def symbols_def)
+  apply (rule Abs_alphabet_induct)
+  apply (auto simp add: alphabet_def)
+  apply (smt Abs_alphabet_inverse CollectI Collect_empty_eq Collect_mem_eq UnI1 alphabet_def)
+  apply (smt Abs_alphabet_inverse CollectI Collect_empty_eq Collect_mem_eq UnI2 alphabet_def)
+  by (smt Abs_alphabet_cases Abs_alphabet_inverse CollectI Collect_empty_eq Collect_mem_eq UnE alphabet_def)
+
+lemma funs_exist: "funs \<Sigma> \<noteq> {}"
+  apply (simp add: funs_def)
+  apply (rule Abs_alphabet_induct)
+  apply (auto simp add: alphabet_def)
+  by (smt CollectE Rep_alphabet alphabet_def)
+
+lemma rels_exist: "rels \<Sigma> \<noteq> {}"
+  apply (simp add: rels_def)
+  apply (rule Abs_alphabet_induct)
+  apply (auto simp add: alphabet_def)
+  by (smt CollectE Rep_alphabet alphabet_def)
+
+end
