Carrier/Trace.thy
@@ -1,0 +1,96 @@
+theory Trace
+  imports Flowchart Quantale
+begin
+
+definition (in alph) atomic_programs :: "flow set" where
+  "atomic_programs = {UNDEFINED, SKIP} \<union> {A. \<exists>x y. A = x y}"
+
+definition (in alph) atomic_tests :: "atomic_formula set" where
+  "atomic_tests = {t. wf_atomic_formula \<Sigma>l t}"
+
+locale kripke_frame = fixes A (structure)
+  fixes tests_map :: "atomic_formula \<Rightarrow> 'a set"
+  and programs_map :: "flow set \<Rightarrow> ('a \<times> 'a) set"
+  and \<Sigma>l :: alphabet
+  assumes tests_map_type: "tests_map : atomic_tests \<rightarrow> Pow (carrier A)"
+  and programs_map_type: "programs_map : atomic_programs \<rightarrow> Pow (carrier A \<times> carrier A)"
+
+sublocale kripke_frame \<subseteq> alph .
+
+datatype 'a trace = tlink 'a "flow set" "'a trace" | tend 'a
+
+context kripke_frame
+begin
+
+  fun wf_trace :: "'a trace \<Rightarrow> bool" where
+    "wf_trace (tlink u0 p0 (tlink u1 p1 \<sigma>)) = ((u0, u1) \<in> programs_map p0 \<and> wf_trace (tlink u1 p1 \<sigma>))"
+  | "wf_trace (tlink u0 p0 (tend u1))       = ((u0, u1) \<in> programs_map p0)"
+  | "wf_trace (tend u1)                     = True"
+
+  fun first :: "'a trace \<Rightarrow> 'a" where
+    "first (tlink u p \<sigma>) = u"
+  | "first (tend u)      = u"
+
+  fun last :: "'a trace \<Rightarrow> 'a" where
+    "last (tlink u p \<sigma>) = last \<sigma>"
+  | "last (tend u)      = u"
+
+  fun join_traces :: "'a trace \<Rightarrow> 'a trace \<Rightarrow> 'a trace" where
+    "join_traces (tlink u p \<sigma>) \<tau> = tlink u p (join_traces \<sigma> \<tau>)"
+  | "join_traces (tend u) \<tau> = \<tau>"
+
+  definition join_trace_sets :: "'a trace set \<Rightarrow> 'a trace set \<Rightarrow> 'a trace set" where
+    "join_trace_sets X Y = {Z. \<exists>\<sigma>\<in>X. \<exists>\<tau>\<in>Y. Z = join_traces \<sigma> \<tau> \<and> last \<sigma> = first \<tau>}"
+
+  definition canonical_program :: "flow set \<Rightarrow> 'a trace set" ("\<lbrace>_\<rbrace>") where
+    "\<lbrace>S\<rbrace> = {\<sigma>. \<exists>u0 u1. \<sigma> = tlink u0 S (tend u1) \<and> (u0, u1) \<in> programs_map S}"
+
+  definition canonical_test :: "atomic_formula \<Rightarrow> 'a trace set" ("\<lbrace>_\<rbrace>") where
+    "\<lbrace>p\<rbrace> = tend ` tests_map p"
+
+  definition all_tests :: "'a trace set" where
+    "all_tests = tend ` UNIV"
+
+  lemma join_trace_onel: "join_trace_sets all_tests X = X"
+    by (auto simp add: join_trace_sets_def all_tests_def)
+
+  lemma join_trace_oner: "join_trace_sets X all_tests = X"
+    apply (auto simp add: join_trace_sets_def all_tests_def)
+  proof -
+    fix \<sigma> :: "'a trace" assume "\<sigma> \<in> X"
+    thus "join_traces \<sigma> (tend (last \<sigma>)) \<in> X"
+      by (induct \<sigma> arbitrary: X, auto)
+    from `\<sigma> \<in> X` show "\<exists>\<tau>\<in>X. \<sigma> = join_traces \<tau> (tend (local.last \<tau>))"
+      by (rule_tac x = \<sigma> in bexI, induct \<sigma> arbitrary: X, auto)
+  qed
+
+  lemma join_traces_assoc:
+    "join_trace_sets (join_trace_sets X Y) Z = join_trace_sets X (join_trace_sets Y Z)"
+    sorry
+
+  abbreviation traces :: "('a trace set) mult_ord" where
+    "traces \<equiv> \<lparr>carrier = UNIV, le = op \<subseteq>, one = all_tests, mult = join_trace_sets\<rparr>"
+
+  lemma traces_ord: "order traces"
+    by (auto simp add: order_def)
+
+  lemma traces_lub [simp]: "\<Sigma>\<^bsub>traces\<^esub> X = \<Union> X"
+    apply (simp add: order.lub_simp[OF traces_ord])
+    apply (rule the1I2)
+    apply (safe, blast, blast)
+    apply (metis in_mono)
+    by blast+
+
+  lemma "unital_quantale traces"
+    apply (simp add: unital_quantale_def, intro conjI)
+    apply unfold_locales
+    apply (simp_all add: order.is_lub_simp[OF traces_ord] order.is_glb_simp[OF traces_ord])
+    apply blast+
+    apply (metis UNIV_I typed_abstraction)
+    apply (metis join_traces_assoc)
+    defer defer
+    apply (metis join_trace_onel)
+    apply (metis join_trace_oner)
+    by (auto simp add: join_trace_sets_def all_tests_def)
+
+end
